Lamcalc/Typed.lean
@@ -3,26 +3,26 @@ import Lamcalc.Confluence
 
 mutual
 inductive Typed : Ctx -> Tm -> Tm -> Prop where
-  | srt Γ (i : Nat) :
+  | srt :
     Wf Γ ->
     Typed Γ (Tm.srt i) (Tm.srt i.succ)
-  | var Γ x a :
+  | var :
     Wf Γ ->
     Has Γ x a ->
     Typed Γ (.var x) a
-  | pi Γ a b i1 i2 :
+  | pi :
     Typed Γ a (Tm.srt i1) ->
     Typed (a :: Γ) b (Tm.srt i2) ->
     Typed Γ (Tm.pi a b) (Tm.srt (max i1 i2))
-  | lam Γ a b m i :
+  | lam :
     Typed Γ a (Tm.srt i) ->
     Typed (a :: Γ) m b ->
     Typed Γ (Tm.lam a m) (Tm.pi a b)
-  | app Γ a b m n :
+  | app :
     Typed Γ m (Tm.pi a b) ->
     Typed Γ n a ->
     Typed Γ (Tm.app m n) (b.[n/])
-  | conv Γ a b m :
+  | conv :
     a === b ->
     Typed Γ m a ->
     Typed Γ b (Tm.srt i) ->
@@ -30,11 +30,13 @@ inductive Typed : Ctx -> Tm -> Tm -> Prop where
 
 inductive Wf : Ctx -> Prop  where
   | nil : Wf []
-  | cons Γ a i :
+  | cons :
+    Wf Γ ->
     Typed Γ a (.srt i) ->
     Wf (a :: Γ)
 end
 
-theorem typed_wf : Typed Γ m a -> Wf Γ  := by
+theorem Typed.wf : Typed Γ m a -> Wf Γ  := by
   intro h
-  induction h using @Typed.rec _ (fun _ _ => True) <;> trivial
+  induction h using Typed.rec (motive_2 := fun _ _ => True)
+  all_goals trivial
