Lamcalc/Weak.lean
@@ -1,0 +1,118 @@
+import Lamcalc.Typed
+
+inductive AgreeRen : (Var -> Var) -> Ctx -> Ctx -> Prop where
+  | nil :
+    AgreeRen ξ  [] []
+  | cons :
+    Typed Γ a (Tm.srt i) ->
+    AgreeRen ξ Γ Γ' ->
+    AgreeRen (upren ξ) (a :: Γ) (a.[ren ξ] :: Γ')
+  | wk :
+    Typed Γ' a (Tm.srt i) ->
+    AgreeRen ξ Γ Γ' ->
+    AgreeRen (ξ >>> Nat.succ) Γ (a :: Γ')
+
+theorem AgreeRen.refl : Wf Γ -> AgreeRen id Γ Γ := by
+  intro wf
+  induction wf using Wf.rec (motive_1 := fun Γ _ _ _ => True)
+  all_goals try trivial
+  case nil => constructor
+  case cons Γ a i ty ih _ =>
+    have h := AgreeRen.cons ty ih
+    asimp at h
+    assumption
+
+theorem AgreeRen.has :
+  AgreeRen ξ Γ Γ' -> Has Γ x a -> Has Γ' (ξ x) a.[ren ξ] := by
+  intro agr
+  induction agr generalizing x a with
+  | nil => intro h; cases h
+  | @cons _ a _ ξ _ _ _ ih =>
+    intro h
+    cases h <;> asimp
+    case zero =>
+      have e : a.[@ren Tm _ ξ >> shift] = a.[ren ξ].[shift] := by asimp
+      rw[e]; constructor
+    case succ x a hs =>
+      have e : a.[@ren Tm _ ξ >> shift] = a.[ren ξ].[shift] := by asimp
+      rw[e]; constructor
+      apply ih; assumption
+  | @wk _ a _ ξ _ _ _ ih =>
+    intro h; asimp
+    have e : a.[@ren Tm _ (ξ >>> Nat.succ)] = a.[ren ξ].[shift] := by asimp; rfl
+    rw[e]; constructor
+    apply ih; assumption
+
+theorem AgreeRen.wf_nil : AgreeRen ξ [] Γ' -> Wf Γ' := by
+  intro agr
+  cases agr with
+  | nil => constructor
+  | wk ty agr =>
+    constructor
+    . apply ty.wf
+    . assumption
+
+theorem AgreeRen.wf_cons :
+  AgreeRen ξ (a :: Γ) Γ' -> Wf Γ ->
+  (∀ Γ' ξ, AgreeRen ξ Γ Γ' → Wf Γ') ->
+  (∀ Γ' ξ, AgreeRen ξ Γ Γ' → ∃ i, Typed Γ' a.[ren ξ] (.srt i)) ->
+  Wf Γ' := by
+  intro agr
+  cases agr with
+  | cons ty agr =>
+    intro wf h1 h2
+    have ⟨i, ty⟩ := h2 _ _ agr
+    constructor
+    . apply h1; assumption
+    . assumption
+  | wk ty agr =>
+    intros
+    constructor
+    . exact ty.wf
+    . assumption
+
+theorem Typed.rename :
+  Typed Γ m A -> AgreeRen ξ Γ Γ' -> Typed Γ' m.[ren ξ] A.[ren ξ] := by
+  intro ty
+  induction ty
+  using Typed.rec (motive_2 := fun Γ _ => ∀ Γ' ξ, AgreeRen ξ Γ Γ' -> Wf Γ')
+  generalizing ξ Γ'
+  with
+  | srt wf ih =>
+    intro; asimp; constructor
+    apply ih; assumption
+  | var wf hs ih =>
+    intro; asimp; constructor
+    . apply ih; assumption
+    . apply AgreeRen.has <;> assumption
+  | pi tya tyb iha ihb =>
+    intro agr; asimp; constructor
+    . apply iha; assumption
+    . have ty := ihb (AgreeRen.cons tya agr)
+      asimp at ty; assumption
+  | lam tya tym iha ihm =>
+    intro agr; asimp; constructor
+    . apply iha; assumption
+    . have ty := ihm (AgreeRen.cons tya agr)
+      asimp at ty; assumption
+  | @app _ m a b n tym tyn ihm ihn =>
+    intro agr; asimp
+    replace tym := ihm agr; asimp at tym
+    replace tyn := ihn agr; asimp at tyn
+    have ty := Typed.app tym tyn; asimp at ty
+    assumption
+  | conv eq tym tyb iha ihb =>
+    intro agr
+    apply Typed.conv
+    . apply Conv.subst; assumption
+    . apply iha; assumption
+    . asimp at ihb; apply ihb; assumption
+  | nil Γ' ξ agr =>
+    exact agr.wf_nil
+  | @cons _ _ i _ _ _ ih _ _ agr =>
+    apply agr.wf_cons
+    . assumption
+    . assumption
+    . intros
+      exists i
+      apply ih; assumption
